lambda2Gmu/CanonicalForms.v
@@ -4,14 +4,38 @@ Require Import TLC.LibTactics.
 Require Import TLC.LibEnv.
 Require Import TLC.LibLN.
 
+  (* Ht : {Σ, empty}⊢ trm_constructor Tparams Name e1 ∈ T1 ** T2 *)
+Lemma CanonicalConstructorType : forall Σ E Tparams Name Ctor e1 T,
+    {Σ, E} ⊢ trm_constructor Tparams (Name, Ctor) e1 ∈ T ->
+    (* TODO can we make Typs more specific? *)
+    exists Typs, T = typ_gadt Typs Name.
+  introv Htyp.
+Admitted.
+
+Lemma CanonicalConstructorTypeGen : forall Σ E Tparams Ctor e1 T,
+    {Σ, E} ⊢ trm_constructor Tparams Ctor e1 ∈ T ->
+    (* TODO can we make Typs more specific? *)
+    exists Typs Name, T = typ_gadt Typs Name.
+  intros.
+  destruct Ctor.
+  apply CanonicalConstructorType in H.
+  destruct H as [Typs Heq].
+  eexists. eexists. eauto.
+Qed.
+
+Hint Resolve CanonicalConstructorTypeGen.
+
 Lemma CanonicalFormTuple : forall Σ e T1 T2,
     value e ->
     {Σ, empty} ⊢ e ∈ T1 ** T2 ->
     exists v1 v2, e = trm_tuple v1 v2.
   introv.
   intros Hv Ht.
-  inversion Hv; inversion Ht; subst; eauto; congruence.
-Qed.
+  inversion Hv; inversion Ht; subst; eauto; try congruence.
+  -
+    admit.
+  (*  An inversion lemma that detects impossible GADTs would be useful  *)
+Admitted.
 
 Lemma CanonicalFormAbs : forall Σ e T1 T2,
     value e ->
@@ -19,8 +43,9 @@ Lemma CanonicalFormAbs : forall Σ e T1 T2,
     exists v1, e = trm_abs T1 v1.
   introv.
   intros Hv Ht.
-  inversion Hv; inversion Ht; subst; eauto; congruence.
-Qed.
+  inversion Hv; inversion Ht; subst; eauto; try congruence.
+  - admit.
+Admitted.
 
 Lemma CanonicalFormTAbs : forall Σ e T,
     value e ->
@@ -28,8 +53,9 @@ Lemma CanonicalFormTAbs : forall Σ e T,
     exists v1, e = trm_tabs v1.
   introv.
   intros Hv Ht.
-  inversion Hv; inversion Ht; subst; eauto; congruence.
-Qed.
+  inversion Hv; inversion Ht; subst; eauto; try congruence.
+  - admit.
+Admitted.
 
 Lemma CanonicalFormUnit : forall Σ e,
     value e ->
@@ -37,5 +63,6 @@ Lemma CanonicalFormUnit : forall Σ e,
     e = trm_unit.
   introv.
   intros Hv Ht.
-  inversion Hv; inversion Ht; subst; eauto; congruence.
-Qed.
+  inversion Hv; inversion Ht; subst; eauto; try congruence.
+  - admit.
+Admitted.
